certicoq/theories/L1_5_box/L1_5.v
@@ -1,0 +1,4 @@
+(** Collect all of L1 together **)
+
+Require Export L1_5.compile.
+Require Export L1_5.term L1_5.program L1_5.wndEval L1_5.wcbvEval L1_5.wNorm.
