certicoq/theories/L2_typeStripped/L2.v
@@ -1,6 +1,7 @@
 (** Collect all of L2 together **)
 
+Add LoadPath "../L2_typeStripped" as L2.
 
-
+Require Export L2.compile.
 Require Export L2.term L2.program L2.wndEval L2.wcbvEval L2.wNorm.
 Require Export L2.stripEvalCommute.
