certicoq/theories/L3_flattenedApp/test_wcbvEval.v
@@ -1,7 +1,7 @@
 (******)
 Add LoadPath "../common" as Common.
 Add LoadPath "../L1_MalechaQuoted" as L1.
-Add LoadPath "../L2_typeStrippedL1" as L2.
+Add LoadPath "../L2_typeStripped" as L2.
 Add LoadPath "../L3_flattenedApp" as L3.
 (******)
 
